
\exercise{Simple change of variables}{1}
Consider the system 
\eqan{
\dot{x}&=&2x-3y \\
\dot{y}&=&xy
}
Rewrite the system in terms of $x$ and the new variable $s=x+y$

\solution
We start with
\eq{
s=x+y 
}
Differentiating with respect to time yields
\eq{
\dot{s}=\dot{x}+\dot{y}
}
Substituting the equations for the time derivatives we find
\eq{
\dot{s}=2x-3y+xy
}
Do the system is now
\eqa{
\dot{x}&=&2x-3y \\
\dot{s}&=&2x-3y+xy
}
To replace the instances of $y$ we solve $s=x+y$ for 
\eq{
y=s-x
}
Substituting into the system we find
\eqa{
\dot{x}&=&2x-3(s-x) \\
\dot{s}&=&2x-3(s-x)+x(s-x)
}
which we can simplify to 
\eqa{
\dot{x}&=&5x-3s \\
\dot{s}&=&5x-3s+xs-x^2
}