
\exercise{Quadratic polynomials}{1}
\label{exBeesQuadratics}
Solve the following quadratic polynomials:
\subquestion $1+\lambda=\lambda^2$,

\solution 
We solve this as 
\eqa{ 
  \lambda^2-\lambda &=& 1 \\
  \lambda^2-\lambda+1/4-1/4  &=& 1 \\
  (\lambda-1/2)^2  &=& 5/4 \\
  \lambda - 1/2    &=& \pm \sqrt{5/4}
}
The result can be written as 
\eq{
\lambda= \frac{1\pm \sqrt{5}}{2}
}

\subquestion $(6-\lambda)(2-\lambda)-60=0$,

\solution 
Unfortunately we need to multiply this out
\eqa{
\lambda^2 - 8 \lambda +12 -60 &=& 0 \\
(\lambda -4 )^2 +12 -60 -16 &=& 0 \\
(\lambda -4 )^2  &=& 64 \\
\lambda-4 &=& \pm 8
}
Hence we find the two solutions $\lambda_1 = -4$ and $\lambda_2=12$

\subquestion $(2-\lambda)^2-9=0$.

\solution 
This one is convenient as we already have a quadratic expression. So straight away 
\eqa{
  (2-\lambda)^2 &=& 9  \\
  \lambda-2 &=& \pm 3
}
and hence $\lambda_1=5$ and $\lambda_2=-1$.

\solutionend